PMapHelperLemmas.v
@@ -2,6 +2,9 @@ From MyProject Require Import SmtExpr.
 From MyProject Require Import CrProgramState.
 From MyProject Require Import CrSymbolicSemanticsTransformer.
 From MyProject Require Import Maps.
+From MyProject Require Import UtilLemmas.
+Require Import Coq.Lists.List.
+Require Import ZArith.
 
 Transparent lookup_ctrl.
 Lemma commute_lookup_eval_ctrl:
@@ -34,6 +37,51 @@ Lemma commute_lookup_eval_state:
 Proof.
   intros.
   apply PMap.gmap.
+Qed.
+
+
+Lemma ptree_of_list_lemma_generic:
+    forall (X : Type) (get_key : X -> positive)
+    (make_item : positive -> X)
+    (l : list X) (val_fn : X -> SmtArithExpr)
+    (x : X),
+    make_item (get_key x) = x ->
+    injective_contravariant get_key ->
+    Coqlib.list_norepet l ->
+    In x l ->
+    In x (map (fun '(key, _) => make_item key)
+    (PTree.elements (PTree_Properties.of_list (combine (map get_key l) (map val_fn l))))).
+Proof.
+  intros X get_key make_item l val_fn x inverses inj_conv H' H.
+  generalize H as H_in.
+  apply functional_list_helper with (key_fn := get_key) (val_fn := val_fn) in H.
+  intros.
+  remember (fun '(key, _) => make_item key) as f.
+  assert(H_tmp: x =
+          f (get_key x, val_fn (x))). {
+  rewrite Heqf.
+  rewrite inverses.
+  reflexivity. }
+  rewrite H_tmp.
+  apply in_map with (f := f) (x := (get_key x, val_fn x)) (l := (PTree.elements
+  (PTree_Properties.of_list (combine (map get_key l) (map val_fn l))))).
+  remember (get_key x, val_fn x) as pair_val.
+  remember (combine (map get_key l) (map val_fn l)) as l_combined.
+  rewrite Heqpair_val in *.
+  apply PTree.elements_correct with (m := PTree_Properties.of_list l_combined).
+  apply PTree_Properties.of_list_norepet.
+  - rewrite Heql_combined.
+    simpl.
+    rewrite map_combine2.
+    apply Coqlib.list_map_norepet.
+    -- assumption.
+    -- intros.
+       apply inj_conv.
+       assumption.
+  - simpl in H. rewrite Heqf in H_tmp.
+    rewrite H_tmp.
+    rewrite inverses.
+    assumption.
 Qed.
 
 Global Opaque lookup_hdr.
